

$$\frac{}{\langle K, \langle \text{null}, \text{Iterator}(\text{s.roots}) \rangle :: [] \rangle}$$

initialConf

$$\frac{\langle K, \langle \text{s}, \text{it} \rangle :: S \rangle \wedge \text{!it.hasNext}}{\langle K, S \rangle}$$

backtrack(c)

$$\frac{\langle K, \langle \text{s}, \text{it} \rangle :: S \rangle \wedge \text{it.hasNext} \wedge (\text{n} = \text{it.peek}) \in K}{\langle K, \langle \text{s}, \text{it.next} \rangle :: S \rangle \rangle}$$

known(n)

$$\frac{\langle K, \langle \text{s}, \text{it} \rangle :: S \rangle \wedge \text{it.hasNext} \wedge (\text{n} = \text{it.peek}) \notin K}{\langle K \cup \{\text{n}\}, \langle \text{n}, \text{Iterator}(\text{s.neighbors}(\text{n})) \rangle :: \langle \text{s}, \text{it.next} \rangle :: S \rangle \rangle}$$

unknown(n)

$$\frac{\langle K, [] \rangle}{\langle K, [] \rangle}$$

end